src/core/DY.Core.Label.fst
@@ -309,11 +309,18 @@ let state_pred_label p = mk_label {
   is_corrupt_later = (fun tr1 tr2 -> ());
 }
 
+val state_pred_label_pred_implies:
+  (principal -> state_id -> bytes -> prop) ->
+  (principal -> state_id -> bytes -> prop) ->
+  prop
+let state_pred_label_pred_implies p1 p2 =
+  forall p s c. p2 p s c ==> p1 p s c
+
 val state_pred_label_can_flow_state_pred_label:
   tr:trace ->
   p1:(principal -> state_id -> bytes -> prop) -> p2:(principal -> state_id -> bytes -> prop) ->
   Lemma
-  (requires forall p s c. p2 p s c ==> p1 p s c)
+  (requires state_pred_label_pred_implies p1 p2)
   (ensures state_pred_label p1 `can_flow tr` state_pred_label p2)
   [SMTPat (state_pred_label p1 `can_flow tr` state_pred_label p2)]
 let state_pred_label_can_flow_state_pred_label tr p1 p2 =
@@ -341,8 +348,8 @@ let is_corrupt_state_pred_label tr p time prin sess_id content =
 val principal_label_pred:
   principal ->
   principal -> state_id -> bytes -> prop
-let principal_label_pred prin1 =
-  fun prin2 _ _ -> prin1 == prin2
+let principal_label_pred prin1 prin2 _ _ =
+  prin1 == prin2
 
 val principal_label: principal -> label
 let principal_label prin =
@@ -351,8 +358,8 @@ let principal_label prin =
 val principal_state_label_pred:
   principal -> state_id ->
   principal -> state_id -> bytes -> prop
-let principal_state_label_pred prin1 sess_id1 =
-  fun prin2 sess_id2 _ -> prin1 == prin2 /\ sess_id1 == sess_id2
+let principal_state_label_pred prin1 sess_id1 prin2 sess_id2 _ =
+  prin1 == prin2 /\ sess_id1 == sess_id2
 
 val principal_state_label: principal -> state_id -> label
 let principal_state_label prin sess_id =
@@ -361,8 +368,8 @@ let principal_state_label prin sess_id =
 val principal_state_content_label_pred:
   principal -> state_id -> bytes ->
   principal -> state_id -> bytes -> prop
-let principal_state_content_label_pred prin1 sess_id1 content1 =
-  fun prin2 sess_id2 content2 -> prin1 == prin2 /\ sess_id1 == sess_id2 /\ content1 == content2
+let principal_state_content_label_pred prin1 sess_id1 content1 prin2 sess_id2 content2 =
+  prin1 == prin2 /\ sess_id1 == sess_id2 /\ content1 == content2
 
 val principal_state_content_label: principal -> state_id -> bytes -> label
 let principal_state_content_label prin sess_id content =
